Working on type substitution in Theory
Having typing lemma completed with additional condition on patterns
Some cases done in term rep lemma
	have lemma for arg_lists
But problem with names and substitution, need stronger well-formed
notion that ensures we can't have name clashes
Formalized predicates holding recursively on term/fmla, prove
equivalent to subterm formulation
Plan to prove that strong well-formed implies recursive well-formed
Then can alpha convert, use strong-well-formed assumption without
losing anything

proofs/core/Theory.v
@@ -866,6 +866,104 @@ Ltac check_theory :=
   apply /check_typed_theory_correct;
   reflexivity.
 
+(*TODO: change in Denotational (generalize params)*)
+Definition get_arg_list {gamma} (gamma_valid: valid_context gamma) 
+  pd (v: val_typevar)
+  (s: fpsym) (vs: list vty) (ts: list term) 
+  (reps: forall (t: term) (ty: vty),
+    term_has_type gamma t ty ->
+    domain (dom_aux pd) (v_subst v ty))
+  {args: list vty}
+  {params: list typevar}
+  (Hp: NoDup params)
+  (Hlents: length ts = length args)
+  (Hlenvs: length vs = length params)
+  (Hall: Forall (fun x => term_has_type gamma (fst x) (snd x))
+    (combine ts (map (ty_subst params vs) args))):
+    arg_list (domain (dom_aux pd))
+    (ty_subst_list_s params
+      (map (v_subst v) vs) args).
+Proof.
+  generalize dependent args. induction ts; simpl; intros.
+  - destruct args.
+    + exact (@HL_nil _ _).
+    + exact (False_rect _ (Nat.neq_0_succ (length args) Hlents)).
+  - destruct args as [| a1 atl].
+    + exact ( False_rect _ (Nat.neq_succ_0 (length ts) Hlents)).
+    + exact ((HL_cons _ _ _ (dom_cast (dom_aux pd)
+    (funsym_subst_eq params vs v a1
+    Hp (Logic.eq_sym Hlenvs))
+      (reps _ _ (Forall_inv Hall)))
+       (IHts atl (*atl*) 
+        (Nat.succ_inj (length ts) (length atl) Hlents)
+        (Forall_inv_tail Hall)))).
+Defined.
+
+(*TODO: change in Denotational (strict generalization)*)
+
+Lemma get_arg_list_vt_ext' {gamma} (gamma_valid: valid_context gamma) 
+pd (pf: pi_funpred gamma_valid pd) 
+(vt1 vt2: val_typevar) (s: fpsym)
+  (vs1 vs2: list vty) (ts1 ts2: list term) vv1 vv2
+  (reps1 reps2: forall (vt: val_typevar) (pf: pi_funpred gamma_valid pd) 
+    (vv: val_vars pd vt)
+    (t: term) (ty: vty) (Hty: term_has_type gamma t ty),
+    domain (dom_aux pd) (v_subst vt ty))
+  (Hts: length ts1 = length ts2)
+  (Hreps: forall (i: nat),
+    (i < length ts1)%coq_nat ->
+    forall (ty1 ty2: vty) Hty1 Hty2 Heq,
+      dom_cast (dom_aux pd) Heq 
+        (reps1 vt1 pf vv1 (List.nth i ts1 tm_d) ty1 Hty1) =
+      reps2 vt2 pf vv2 (List.nth i ts2 tm_d) ty2 Hty2)
+  {args: list vty}
+  {params: list typevar}
+  (Hp: NoDup params)
+  (Hlents1: length ts1 = length args)
+  (Hlents2: length ts2 = length args)
+  (Hlenvs1: length vs1 = length params)
+  (Hlenvs2: length vs2 = length params)
+  (Hall1: Forall (fun x => term_has_type gamma (fst x) (snd x))
+    (combine ts1 (map (ty_subst params vs1) args)))
+  (Hall2: Forall (fun x => term_has_type gamma (fst x) (snd x))
+    (combine ts2 (map (ty_subst params vs2) args)))
+  (Heq: map (v_subst vt1) vs1 = map (v_subst vt2) vs2):
+  cast_arg_list 
+    (f_equal (fun x => ty_subst_list_s params x args) Heq)
+    (get_arg_list gamma_valid pd vt1 s vs1 ts1 (reps1 vt1 pf vv1) Hp Hlents1 Hlenvs1 Hall1) =
+  get_arg_list gamma_valid pd vt2 s vs2 ts2 (reps2 vt2 pf vv2) Hp Hlents2 Hlenvs2 Hall2.
+Proof.
+  match goal with
+  | |- cast_arg_list ?H ?a = _ => generalize dependent H end.
+  clear Heq.
+  unfold get_arg_list.
+  generalize dependent args.
+  generalize dependent ts2. 
+  induction ts1; simpl; intros. 
+  - destruct ts2; [|subst; inversion Hts].
+    destruct args; simpl; auto; [|inversion Hlents1].
+    assert (e = Logic.eq_refl). apply UIP_dec. apply list_eq_dec.
+    apply sort_eq_dec. 
+    subst. reflexivity.
+  - destruct ts2; inversion Hts.
+    destruct args.
+    + inversion Hlents2.
+    + simpl in Hlenvs2. simpl.
+      simpl in e.
+      rewrite (cast_arg_list_cons e).
+      f_equal.
+      * rewrite -> rewrite_dom_cast, !dom_cast_compose.
+        assert (Heq': v_subst vt1 (ty_subst params vs1 v) = v_subst vt2 (ty_subst params vs2 v)). {
+          rewrite !funsym_subst_eq; auto.
+          apply (cons_inj_hd e).
+        }
+        erewrite <- (Hreps 0) with(Hty1:=Forall_inv Hall1)(Heq:=Heq'); try lia.
+        rewrite !dom_cast_compose. apply dom_cast_eq.
+      * apply IHts1; auto.
+        intros i Hi ty Hty1 Hty2 Heq.
+        apply (Hreps (S i) (ltac:(lia))).
+Qed.
+
 (*This defines what it means for a theory
   to be valid.
   We want to do the following
@@ -879,6 +977,1518 @@ Ltac check_theory :=
     then (theory_ctx_int t, theory_axioms t) |= f
     and as a corollary, if no axioms, then gamma, . |= f
     (more of a sanity check than anything else)*)
+
+(*Monomoprhize goals if polymorphic*)
+
+(*To prove that patterns are well-typed,
+  we need a condition that the names of pattern variables
+  are unique (not just the vsymbols). Really, this should
+  be in typing, but it makes alpha equvialence much harder.
+  For now, we have a separate condition, which we can check.
+  We could alpha convert if needed to make this condition true*)
+(*Give as bool*)
+Section PatUniq.
+
+Fixpoint pat_names_uniq (p:pattern) : Prop :=
+  match p with
+  | Pconstr f args ps =>
+    Forall id (map pat_names_uniq ps) /\
+    forall i j, (i < length ps)%coq_nat -> (j < length ps)%coq_nat ->
+    i <> j ->
+    forall x, ~ (In x (map fst (pat_fv (List.nth i ps Pwild))) /\
+      In x (map fst (pat_fv (List.nth j ps Pwild))))
+  | Por p1 p2 => pat_names_uniq p1 /\ pat_names_uniq p2
+  | Pbind p x => pat_names_uniq p /\ ~ In (fst x) (map fst (pat_fv p))
+  | _ => true
+  end.
+
+Fixpoint pat_names_uniqb (p: pattern) : bool :=
+  match p with
+  | Pconstr f args ps => 
+    all id (map pat_names_uniqb ps) &&
+    [forall x in 'I_(length ps), forall y in 'I_(length ps),
+    (x != y) ==>  
+    null (seqI (map fst (pat_fv (nth Pwild ps x))) 
+      (map fst (pat_fv (nth Pwild ps y))))]
+  | Por p1 p2 => pat_names_uniqb p1 && pat_names_uniqb p2
+  | Pbind p x => pat_names_uniqb p && 
+    ((fst x) \notin (map fst (pat_fv p)))
+  | _ => true
+  end.
+
+Lemma all_Forall_idP {A: Type} (P: A -> Prop) (b: A -> bool)
+  (l: list A):
+  (forall x, In x l -> reflect (P x) (b x)) ->
+  reflect (Forall id (map P l)) (all id (map b l)).
+Proof.
+  move=>Hrefl.
+  apply iff_reflect. rewrite Forall_map all_map.
+  apply reflect_iff.
+  apply forallb_ForallP => x Hinx.
+  by apply Hrefl.
+Qed.
+
+Lemma pat_names_uniqb_correct p:
+  reflect (pat_names_uniq p) (pat_names_uniqb p).
+Proof.
+  apply 
+    (pattern_rect (fun (p: pattern) => 
+      reflect (pat_names_uniq p) (pat_names_uniqb p)))=>//=.
+  - move=> _. by reflT.
+  - (*The hard case*)
+    move=> f vs ps Hall.
+    have Hallr: reflect (Forall id [seq pat_names_uniq i | i <- ps])
+      (all id [seq pat_names_uniqb i | i <- ps]).
+    {
+      apply all_Forall_idP.
+      apply ForallT_In=>//. apply pattern_eq_dec. 
+    }
+    case: Hallr => Halluniq; last by reflF.
+    case: [forall x in 'I_(Datatypes.length ps),
+    forall y in 'I_(Datatypes.length ps),
+    (x != y) ==>
+    null (seqI (map fst(pat_fv (nth Pwild ps x))) 
+      (map fst (pat_fv (nth Pwild ps y))))] 
+    /forallP => Hforallx/=; last first.
+    + apply ReflectF => [[_ C]]. apply Hforallx. move=> x.
+      apply /implyP => _. apply /forallP => y.
+      apply /implyP=>_. apply /implyP => Hneq.
+      apply /nullP. apply /eqP. 
+      rewrite /seqI -(negbK (_ == _)) -has_filter. 
+      apply /negP => /hasP [z] /inP Hzin1 /inP Hzin2.
+      apply (C x y (ltac:(by apply /ltP)) (ltac:(by apply /ltP))
+        (ltac:(by apply /eqP)) z).
+      by rewrite !nth_eq.
+    + apply ReflectT. split=>//. move => i j /ltP Hi /ltP Hj /eqP Hij x.
+      rewrite !nth_eq => [[Hinxi Hinxj]].
+      move: Hforallx => /(_ (Ordinal Hi))/= /forallP 
+        /(_ (Ordinal Hj))/= /implyP.
+      have Hneq: (Ordinal (n:=Datatypes.length ps) (m:=i) Hi
+        != Ordinal (n:=Datatypes.length ps) (m:=j) Hj).
+      apply /eqP=> C. inversion C; subst. by rewrite eq_refl in Hij.
+      move=>/(_ Hneq) /nullP /eqP. 
+      rewrite /seqI -(negbK (_ == _)) -has_filter => /hasP.
+      apply. by exists x; apply /inP.
+  - by reflT.
+  - move=> p1 p2 Hr1 Hr2. by apply andPP.
+  - move=> p1 v Hr.
+    apply andPP=>//.
+    apply negPP. apply inP.
+Qed.
+
+(*Push through terms and formulas*)
+Fixpoint pat_names_uniq_t (t: term) : Prop :=
+  match t with
+  | Tfun f tys tms => Forall id (map pat_names_uniq_t tms)
+  | Tlet t1 v t2 => pat_names_uniq_t t1 /\ pat_names_uniq_t t2
+  | Tif f t1 t2 => pat_names_uniq_f f /\ pat_names_uniq_t t1 /\
+    pat_names_uniq_t t2
+  | Tmatch t ty ps => pat_names_uniq_t t /\
+    Forall id (map (fun x => pat_names_uniq (fst x) /\ pat_names_uniq_t (snd x)) ps)
+  | Teps f x => pat_names_uniq_f f
+  | _ => True
+  end
+with pat_names_uniq_f (f: formula) : Prop :=
+  match f with
+  | Fpred p tys tms => Forall id (map pat_names_uniq_t tms)
+  | Fquant q v f => pat_names_uniq_f f
+  | Feq ty t1 t2 => pat_names_uniq_t t1 /\ pat_names_uniq_t t2
+  | Fbinop b f1 f2 => pat_names_uniq_f f1 /\ pat_names_uniq_f f2
+  | Fnot f => pat_names_uniq_f f
+  | Flet t1 v f => pat_names_uniq_t t1 /\ pat_names_uniq_f f
+  | Fif f1 f2 f3 => pat_names_uniq_f f1 /\ pat_names_uniq_f f2 /\
+    pat_names_uniq_f f3
+  | Fmatch t ty ps => pat_names_uniq_t t /\
+    Forall id (map (fun x => pat_names_uniq (fst x) /\ pat_names_uniq_f (snd x)) ps)
+  | _ => True
+  end.
+
+Fixpoint pat_names_uniq_tb (t: term) : bool :=
+  match t with
+  | Tfun f tys tms => all id (map pat_names_uniq_tb tms)
+  | Tlet t1 v t2 => pat_names_uniq_tb t1 && pat_names_uniq_tb t2
+  | Tif f t1 t2 => pat_names_uniq_fb f && pat_names_uniq_tb t1 &&
+    pat_names_uniq_tb t2
+  | Tmatch t ty ps => pat_names_uniq_tb t &&
+    all id (map (fun x => pat_names_uniqb (fst x) && pat_names_uniq_tb (snd x)) ps)
+  | Teps f x => pat_names_uniq_fb f
+  | _ => true
+  end
+with pat_names_uniq_fb (f: formula) : bool :=
+  match f with
+  | Fpred p tys tms => all id (map pat_names_uniq_tb tms)
+  | Fquant q v f => pat_names_uniq_fb f
+  | Feq ty t1 t2 => pat_names_uniq_tb t1 && pat_names_uniq_tb t2
+  | Fbinop b f1 f2 => pat_names_uniq_fb f1 && pat_names_uniq_fb f2
+  | Fnot f => pat_names_uniq_fb f
+  | Flet t1 v f => pat_names_uniq_tb t1 && pat_names_uniq_fb f
+  | Fif f1 f2 f3 => pat_names_uniq_fb f1 && pat_names_uniq_fb f2 &&
+    pat_names_uniq_fb f3
+  | Fmatch t ty ps => pat_names_uniq_tb t &&
+    all id (map (fun x => pat_names_uniqb (fst x) && pat_names_uniq_fb (snd x)) ps)
+  | _ => true
+  end.
+
+Lemma pat_names_uniq_b_correct (t: term) (f: formula):
+  (reflect (pat_names_uniq_t t) (pat_names_uniq_tb t)) *
+  (reflect (pat_names_uniq_f f) (pat_names_uniq_fb f)).
+Proof.
+  revert t f. apply term_formula_rect=>//=.
+  - move=>_. by reflT.
+  - move=>_. by reflT.
+  - move=>_ _ tms Hall.
+    apply all_Forall_idP.
+    apply ForallT_In=>//. apply term_eq_dec.
+  - move=>tm1 _ tm2 Hr1 Hr2.
+    by apply andPP.
+  - move=> f t1 t2 Hr1 Hr2 Hr3.
+    rewrite -andbA.
+    apply andPP=>//.
+    by apply andPP.
+  - move=> t _ ps Hr Hall.
+    apply andPP=>//.
+    apply all_Forall_idP=> x Hinx.
+    apply andPP.
+    + apply pat_names_uniqb_correct.
+    + apply ForallT_In with(x:=snd x) in Hall=>//.
+      apply term_eq_dec. rewrite in_map_iff.
+      by exists x. 
+  - move=>_ _ tms Hall.
+    apply all_Forall_idP.
+    apply ForallT_In=>//. apply term_eq_dec.
+  - move=>_ t1 t2 Hr1 Hr2.
+    by apply andPP.
+  - move=>_ f1 f2 Hr1 Hr2.
+    by apply andPP.
+  - by reflT.
+  - by reflT.
+  - move=>t _ f Hr1 Hr2.
+    by apply andPP.
+  - move=>f1 f2 f3 Hr1 Hr2 Hr3.
+    rewrite -andbA. by repeat apply andPP=>//.
+  - move=> t _ ps Hr Hall.
+    apply andPP=>//.
+    apply all_Forall_idP=> x Hinx.
+    apply andPP.
+    + apply pat_names_uniqb_correct.
+    + apply ForallT_In with(x:=snd x) in Hall=>//.
+      apply formula_eq_dec. rewrite in_map_iff.
+      by exists x.
+Qed. 
+
+End PatUniq.
+
+Section Mono.
+
+(*Idea: extend context with new type symbols, replace
+  each type variable with one of these constants*)
+(*Our type constants will be 'x0, 'x1, etc*)
+Definition tyconstsym (n: string) : typesym :=
+  mk_ts n nil.
+Definition tyconst (n: string) : vty :=
+  vty_cons (tyconstsym n) nil.
+Definition tyconst_s (n: string) : Types.sort :=
+  exist _ (tyconst n) Logic.eq_refl.
+
+(*TODO: move*)
+(*Substitue a type for a type variable in a term/formula*)
+(*Definition ty_subst_single (ty: vty) (a: typevar) (v: vty) :=
+  ty_subst' [a] [ty] v.*)
+
+Definition ty_subst_list' (vs: list typevar) (ts: list vty) (l: list vty) :=
+  map (ty_subst' vs ts) l.
+
+Lemma valid_type_ty_subst': forall s ty vars tys,
+  valid_type s ty ->
+  Forall (valid_type s) tys ->
+  valid_type s (ty_subst' vars tys ty).
+Proof.
+  intros.
+  induction ty; simpl; auto.
+  - destruct (in_dec typevar_eq_dec v vars); auto.
+    apply valid_type_ty_subst; auto.
+  - inversion H; subst. constructor; auto.
+    rewrite map_length; auto.
+    intros x. rewrite in_map_iff. intros [y [Hx Hiny]]; subst.
+    rewrite Forall_forall in H1. apply H1; auto.
+Qed.
+
+Require Import Alpha.
+Section TySubst.
+
+Variable (params: list typevar) (tys: list vty).
+
+Definition ty_subst_var (v: vsymbol) : vsymbol :=
+  (fst v, ty_subst' params tys (snd v)).
+
+(*Definition ty_subst_p := map_pat ty_subst_var.*)
+
+
+
+
+
+
+Fixpoint ty_subst_p (p: pattern) : pattern :=
+  match p with
+  | Pvar x => Pvar (ty_subst_var x)
+  | Pconstr f args ps => Pconstr f (ty_subst_list' params tys args)
+    (map ty_subst_p ps)
+  | Pwild => Pwild
+  | Por p1 p2 => Por (ty_subst_p p1) (ty_subst_p p2)
+  | Pbind p x => Pbind (ty_subst_p p) (ty_subst_var x)
+  end.
+
+Fixpoint ty_subst_tm  (t: term) : term :=
+  match t with
+  | Tconst c => Tconst c
+  | Tvar v => Tvar (ty_subst_var v)
+  | Tfun f args tms =>
+    Tfun f (ty_subst_list' params tys args) (map ty_subst_tm tms)
+  | Tlet t1 x t2 =>
+    Tlet (ty_subst_tm  t1) (ty_subst_var x)
+      (ty_subst_tm t2)
+  | Tif f t1 t2 =>
+    Tif (ty_subst_fmla f) (ty_subst_tm t1) (ty_subst_tm t2)
+  | Tmatch t ty ps =>
+    Tmatch (ty_subst_tm t) (ty_subst' params tys ty)
+    (map (fun x => (ty_subst_p (fst x), ty_subst_tm (snd x))) ps)
+  | Teps f x => Teps (ty_subst_fmla f) (ty_subst_var x)
+  end
+with ty_subst_fmla (f: formula) : formula :=
+  match f with
+  | Fpred p args tms => Fpred p (ty_subst_list' params tys args)
+    (map ty_subst_tm tms)
+  | Fquant q x f => Fquant q (ty_subst_var x) (ty_subst_fmla f)
+  | Feq ty t1 t2 => Feq (ty_subst' params tys ty) (ty_subst_tm t1)
+    (ty_subst_tm t2)
+  | Fbinop b f1 f2 => Fbinop b (ty_subst_fmla f1) (ty_subst_fmla f2)
+  | Fnot f => Fnot (ty_subst_fmla f)
+  | Ftrue => Ftrue
+  | Ffalse => Ffalse 
+  | Flet t x f => Flet (ty_subst_tm t) (ty_subst_var x) (ty_subst_fmla f)
+  | Fif f1 f2 f3 => Fif (ty_subst_fmla f1) (ty_subst_fmla f2)
+    (ty_subst_fmla f3)
+  | Fmatch t ty ps =>
+   Fmatch (ty_subst_tm t) (ty_subst' params tys ty)
+   (map (fun x => (ty_subst_p (fst x), ty_subst_fmla (snd x))) ps)
+  end.
+
+(*Typing*)
+Context {gamma: context} (gamma_valid: valid_context gamma).
+Variable (*(Hnodup: NoDup params) (Hlen: length params = length tys)*)
+  (Hval: Forall (valid_type gamma) tys).
+
+Lemma ty_subst_var_valid (v: vsymbol):
+  valid_type gamma (snd v) ->
+  valid_type gamma (snd (ty_subst_var v)).
+Proof.
+  destruct v; simpl. intros.
+  apply valid_type_ty_subst'; auto.
+Qed.
+
+Lemma ty_subst_twice params1 tys1 params2 tys2 ty:
+  NoDup params1 ->
+  length params1 = length tys1 ->
+  ty_subst' params2 tys2 (ty_subst params1 tys1 ty) =
+  ty_subst params1 (ty_subst_list' params2 tys2 tys1) ty.
+Proof.
+  intros Hn1 Hlen1.
+  unfold ty_subst_list', ty_subst.
+  induction ty; simpl; auto.
+  - destruct (in_dec typevar_eq_dec v params1).
+    + destruct (In_nth _ _ EmptyString i) as [j [Hj Hv]]; subst.
+      rewrite -> !ty_subst_fun_nth with (s:=s_int); auto; [| rewrite map_length; auto].
+      rewrite -> map_nth_inbound with(d2:=vty_int); [| rewrite <- Hlen1; auto].
+      reflexivity.
+    + rewrite !ty_subst_fun_notin; auto. 
+  - f_equal.
+    apply list_eq_ext'; rewrite !map_length; auto.
+    intros n d Hn'.
+    rewrite -> !map_nth_inbound with (d2:=vty_int); auto;
+    [| rewrite map_length; auto].
+    rewrite Forall_forall in H. apply H. apply nth_In; auto.
+Qed.
+
+(*Lemma ty_subst_p_fv (p: pattern):
+  pat_fv (ty_subst_p p) = map ty_subst_var (pat_fv p).
+Proof.
+  induction p; simpl; auto.
+  - induction ps; simpl; intros; auto. inversion H; subst; simpl; auto.
+    Check map_union.
+    rewrite map_union.
+    rewrite union_map. 
+  
+  Search big_union map.*)
+
+Lemma ty_subst_p_fv (p: pattern):
+(forall x, In x (pat_fv (ty_subst_p p)) <-> In x (map ty_subst_var (pat_fv p))).
+Proof.
+  intros. induction p; simpl; auto; try reflexivity.
+  - simpl_set. rewrite in_map_iff.
+    split.
+    + intros [p [Hinp Hinx]].
+      revert Hinp; rewrite in_map_iff.
+      intros [p' [Hpeq Hinp']]; subst.
+      rewrite Forall_forall in H.
+      specialize (H _ Hinp').
+      destruct H. specialize (H Hinx); clear H0.
+      rewrite in_map_iff in H.
+      destruct H as [x' [Hx Hinx']]; subst.
+      exists x'. split; auto. simpl_set.
+      exists p'; auto.
+    + intros [x' [Hx Hinx']]; subst.
+      revert Hinx'. simpl_set. intros [p [Hinp Hinx']].
+      rewrite Forall_forall in H.
+      specialize (H _ Hinp). destruct H.
+      clear H. rewrite in_map_iff in H0.
+      prove_hyp H0.
+      { exists x'. split; auto. }
+      exists (ty_subst_p p); split; auto.
+      rewrite in_map_iff. exists p; auto.
+  - simpl_set. rewrite IHp1 IHp2.
+    rewrite !in_map_iff. split; intros; destruct_all; subst.
+    + exists x0. split; auto; simpl_set; auto.
+    + exists x0. split; auto; simpl_set; auto.
+    + simpl_set. destruct H0; [left | right]; exists x0; auto.
+  - simpl_set. rewrite IHp. rewrite !in_map_iff;
+    split; intros; destruct_all; subst.
+    + exists x0; simpl_set; auto.
+    + exists v; simpl_set; auto.
+    + simpl_set. destruct H0 as [Hinx1 | [Hxv | []]]; subst;
+      [left | right]; auto.
+      exists x0; auto.
+Qed.
+
+Lemma ty_subst_var_fst v1 v2:
+  ty_subst_var v1 = ty_subst_var v2 ->
+  fst v1 = fst v2.
+Proof.
+  unfold ty_subst_var; intros. inversion H; subst; auto.
+Qed.
+    
+Lemma ty_subst_p_ty (p: pattern) (ty: vty)
+  (Hp: pattern_has_type gamma p ty)
+  (Hp2: pat_names_uniq p):
+  pattern_has_type gamma (ty_subst_p p) (ty_subst' params tys ty).
+  (*pat_fv (ty_subst_p p) = map ty_subst_var (pat_fv p).*)
+Proof.
+  generalize dependent ty.
+  induction p; simpl; intros; inversion Hp; subst.
+  - constructor. apply ty_subst_var_valid; auto.
+  - subst sigma. rewrite ty_subst_twice; auto; [| apply s_params_Nodup].
+    constructor; auto.
+    + rewrite Forall_forall. intros x. rewrite in_map_iff.
+      intros [y [Hy Hiny]]; subst.
+      apply valid_type_ty_subst'; auto.
+      rewrite Forall_forall in H4. apply H4; auto.
+    + rewrite map_length; auto.
+    + rewrite map_length; auto.
+    + intros x. rewrite in_combine_iff; rewrite !map_length; auto.
+      intros [i [Hi Hx]]. specialize (Hx Pwild vty_int); subst; simpl.
+      rewrite -> !map_nth_inbound with(d2:=vty_int); try lia.
+      rewrite -> map_nth_inbound with (d2:=Pwild); auto.
+      rewrite Forall_forall in H.
+      rewrite <- ty_subst_twice; auto; [| apply s_params_Nodup].
+      apply H; [apply nth_In; auto| |].
+      * simpl in Hp2. destruct Hp2.
+        rewrite Forall_map in H0.
+        rewrite Forall_forall in H0. apply H0. apply nth_In; auto.
+      * apply (H10 (List.nth i ps Pwild,  (ty_subst (s_params f) vs (List.nth i (s_args f) vty_int)))).
+        rewrite in_combine_iff; try rewrite !map_length; auto.
+        exists i. split; auto. intros.
+        f_equal; try apply nth_indep; auto.
+        rewrite -> map_nth_inbound with (d2:=vty_int); auto; lia.
+    + rewrite !map_length. intros.
+      rewrite -> !map_nth_inbound with (d2:=Pwild); auto.
+      rewrite !ty_subst_p_fv.
+      rewrite -> !in_map_iff; intros [Hex1 Hex2]; destruct_all; subst.
+      (*Here, we need the assumption - types may be same but names cannot*)
+      apply ty_subst_var_fst in H7.
+      simpl in Hp2.
+      destruct Hp2 as [_ Hdisj].
+      apply (Hdisj i j H0 H1 H2 (fst x0)).
+      split; rewrite in_map_iff; [exists x1 | exists x0]; auto.
+  - constructor. apply valid_type_ty_subst'; auto.
+  - simpl in Hp2. destruct Hp2. constructor.
+    + apply IHp1; auto.
+    + apply IHp2; auto.
+    + intros. rewrite !ty_subst_p_fv.
+      rewrite !in_map_iff; split; intros; destruct_all; exists x0;
+      split; auto; apply H5; auto.
+  - simpl in Hp2. destruct Hp2.
+    constructor.
+    + rewrite ty_subst_p_fv in_map_iff; intros C; destruct_all.
+      apply H0. rewrite in_map_iff. exists x; split; auto.
+      apply ty_subst_var_fst; auto.
+    + apply IHp; auto.
+Qed.
+
+Lemma ty_subst_tf_ty (t: term) (f: formula):
+  (forall ty (Hty: term_has_type gamma t ty)
+    (Hp: pat_names_uniq_t t),
+    term_has_type gamma (ty_subst_tm t) (ty_subst' params tys ty)) /\
+  (forall (Hty: formula_typed gamma f)
+    (Hp: pat_names_uniq_f f),
+    formula_typed gamma (ty_subst_fmla f)).
+Proof.
+  revert t f; apply term_formula_ind; simpl; intros; auto;
+  inversion Hty; subst; try solve[unfold ty_subst; simpl; constructor];
+  try solve[destruct_all; constructor; auto;
+    try apply ty_subst_var_valid; auto; solve[intuition]].
+  (*Only Fun/Pred, Match are nontrivial*)
+  - (*Function is tricky case, but simpler than pattern constr*) 
+    rewrite ty_subst_twice; auto; [| apply s_params_Nodup].
+    constructor; auto.
+    + rewrite Forall_forall; intros.
+      unfold ty_subst_list in H0.
+      rewrite in_map_iff in H0. destruct H0 as [ty [Hx Hinty]]; subst.
+      apply valid_type_ty_subst'; auto. rewrite Forall_forall in H4.
+      apply H4; auto.
+    + rewrite map_length; auto.
+    + rewrite map_length; auto.
+    + revert H10 H. rewrite !Forall_forall; intros.
+      revert H0.
+      rewrite in_combine_iff; rewrite !map_length; auto.
+      intros [i [Hi Hx]]; subst. specialize (Hx tm_d vty_int); subst;
+      simpl.
+      rewrite -> !map_nth_inbound with (d2:=vty_int); try lia.
+      rewrite -> !map_nth_inbound with (d2:=tm_d); auto.
+      rewrite <- ty_subst_twice; auto; [| apply s_params_Nodup].
+      apply H; auto.
+      * apply nth_In; auto.
+      * apply (H10 ((nth i l1 tm_d), (ty_subst (s_params f1) l (nth i (s_args f1) vty_int)))).
+        rewrite in_combine_iff; [| rewrite map_length; auto].
+        exists i. split; auto.
+        intros. rewrite -> !map_nth_inbound with (d2:=vty_int); try lia.
+        f_equal. apply nth_indep; auto.
+      * rewrite Forall_map in Hp.
+        rewrite Forall_forall in Hp. apply Hp. apply nth_In; auto.
+  -(*Match relies on pattern typing, rest is easy*) 
+    destruct Hp as [Hpt Hallp].
+    constructor; auto.
+    + destruct H4 as [a [m [args [m_in [a_in Hv]]]]]; subst.
+      exists a. exists m. exists (ty_subst_list' params tys args).
+      split_all; auto.
+    + intros x. rewrite in_map_iff. intros [x1 [Hx Hinx1]]; subst. simpl.
+      apply ty_subst_p_ty; auto. rewrite Forall_map in Hallp.
+      rewrite Forall_forall in Hallp. apply Hallp; auto.
+    + intros x. rewrite in_map_iff. intros [x1 [Hx Hinx1]]; subst; simpl.
+      rewrite Forall_forall in H0.
+      apply H0; auto.
+      * rewrite in_map_iff. exists x1; auto.
+      * rewrite Forall_map Forall_forall in Hallp.
+        apply Hallp; auto.
+    + rewrite null_map. auto.
+  - (*Pred almost same as Fun*) constructor; auto.
+    + rewrite Forall_forall; intros.
+      unfold ty_subst_list in H0.
+      rewrite in_map_iff in H0. destruct H0 as [ty [Hx Hinty]]; subst.
+      apply valid_type_ty_subst'; auto. rewrite Forall_forall in H4.
+      apply H4; auto.
+    + rewrite map_length; auto.
+    + rewrite map_length; auto.
+    + revert H8 H. rewrite !Forall_forall; intros.
+      revert H0.
+      rewrite in_combine_iff; rewrite !map_length; auto.
+      intros [i [Hi Hx]]; subst. specialize (Hx tm_d vty_int); subst;
+      simpl.
+      rewrite -> !map_nth_inbound with (d2:=vty_int); try lia.
+      rewrite -> !map_nth_inbound with (d2:=tm_d); auto.
+      rewrite <- ty_subst_twice; auto; [| apply s_params_Nodup].
+      apply H; auto.
+      * apply nth_In; auto.
+      * apply (H8 ((nth i tms tm_d), (ty_subst (s_params p) tys0 (nth i (s_args p) vty_int)))).
+        rewrite in_combine_iff; [| rewrite map_length; auto].
+        exists i. split; auto.
+        intros. rewrite -> !map_nth_inbound with (d2:=vty_int); try lia.
+        f_equal. apply nth_indep; auto.
+      * rewrite Forall_map in Hp.
+        rewrite Forall_forall in Hp. apply Hp. apply nth_In; auto.
+  - (*Exact same proof*) destruct Hp as [Hpt Hallp].
+    constructor; auto.
+    + destruct H4 as [a [m [args [m_in [a_in Hv]]]]]; subst.
+      exists a. exists m. exists (ty_subst_list' params tys args).
+      split_all; auto.
+    + intros x. rewrite in_map_iff. intros [x1 [Hx Hinx1]]; subst. simpl.
+      apply ty_subst_p_ty; auto. rewrite Forall_map in Hallp.
+      rewrite Forall_forall in Hallp. apply Hallp; auto.
+    + intros x. rewrite in_map_iff. intros [x1 [Hx Hinx1]]; subst; simpl.
+      rewrite Forall_forall in H0.
+      apply H0; auto.
+      * rewrite in_map_iff. exists x1; auto.
+      * rewrite Forall_map Forall_forall in Hallp.
+        apply Hallp; auto.
+    + rewrite null_map. auto.
+Qed.
+
+Definition ty_subst_t_ty t := proj_tm ty_subst_tf_ty t.
+Definition ty_subst_f_ty f := proj_fmla ty_subst_tf_ty f.
+
+(*Part 2: reps for ty substitution.
+  Much like term variable substitution, this corresponds
+  to a change in valuation. Because it changes vt, 
+  this induces annoying cast issues*)
+Print upd_vv_args.
+
+Variable (params_len: length params = length tys)
+  (params_nodup: NoDup params).
+
+Lemma params_len' vt: length params = length (map (v_subst vt) tys).
+Proof.
+  rewrite map_length; auto.
+Qed.
+
+Lemma v_subst_aux_twice f ty:
+  (forall x, is_sort (f x)) ->
+  v_subst_aux f (v_subst_aux f ty) =
+  v_subst_aux f ty.
+Proof.
+  intros Hsort.
+  induction ty; simpl; auto.
+  rewrite <- subst_is_sort_eq; auto.
+  f_equal. rewrite <- map_comp.
+  apply list_eq_ext'; rewrite !map_length; auto.
+  intros n d Hn.
+  rewrite -> !map_nth_inbound with (d2:=vty_int); auto.
+  rewrite Forall_forall in H. apply H.
+  apply nth_In; auto.
+Qed.
+
+Lemma v_subst_vt_with_args' vt (v: vty):
+  v_subst vt (ty_subst' params tys v) =
+  v_subst (vt_with_args vt params (map (v_subst vt) tys)) v.
+Proof.
+  rewrite v_subst_vt_with_args; auto. 2: exact (params_len' _).
+  unfold ty_subst_var. simpl.
+  (*Idea: typevars assigned vt, either now or later*)
+  induction v; simpl; auto.
+  - destruct (in_dec typevar_eq_dec v params); auto.
+    destruct (In_nth _ _ EmptyString i) as [j [Hj Hx]]; subst.
+    apply sort_inj; simpl.
+    unfold ty_subst. simpl.
+    rewrite -> !ty_subst_fun_nth with(s:=s_int); auto;
+    [| rewrite !map_length; auto].
+    unfold sorts_to_tys.
+    rewrite -> !map_nth_inbound with (d2:=s_int);
+    [| rewrite map_length -params_len; auto].
+    rewrite -> map_nth_inbound with (d2:=vty_int);
+    [| rewrite -params_len; auto].
+    simpl.
+    rewrite v_subst_aux_twice; auto.
+    intros. destruct (vt x); auto.
+  - apply sort_inj; simpl. f_equal.
+    rewrite <- !map_comp.
+    apply list_eq_ext'; rewrite !map_length; auto.
+    intros n d Hn.
+    rewrite -> !map_nth_inbound with (d2:=vty_int); auto.
+    rewrite Forall_forall in H.
+    simpl.
+    specialize (H (nth n vs vty_int) (ltac:(apply nth_In; auto))).
+    inversion H; auto.
+Qed.
+(*Lemma v_subst_vt_with_args' vt (x: vsymbol):
+  v_subst vt (ty_subst_var x).2 =
+  v_subst (vt_with_args vt params (map (v_subst vt) tys)) x.2.
+Proof.
+  unfold ty_subst_var. simpl.
+  rewrite v_subst_vt_with_args; auto. 2: exact (params_len' _).
+  unfold ty_subst_var. simpl.
+  (*Idea: typevars assigned vt, either now or later*)
+  induction (x.2); simpl; auto.
+  - destruct (in_dec typevar_eq_dec v params); auto.
+    destruct (In_nth _ _ EmptyString i) as [j [Hj Hx]]; subst.
+    apply sort_inj; simpl.
+    unfold ty_subst. simpl.
+    rewrite -> !ty_subst_fun_nth with(s:=s_int); auto;
+    [| rewrite !map_length; auto].
+    unfold sorts_to_tys.
+    rewrite -> !map_nth_inbound with (d2:=s_int);
+    [| rewrite map_length -params_len; auto].
+    rewrite -> map_nth_inbound with (d2:=vty_int);
+    [| rewrite -params_len; auto].
+    simpl.
+    rewrite v_subst_aux_twice; auto.
+    intros. destruct (vt x0); auto.
+  - apply sort_inj; simpl. f_equal.
+    rewrite <- !map_comp.
+    apply list_eq_ext'; rewrite !map_length; auto.
+    intros n d Hn.
+    rewrite -> !map_nth_inbound with (d2:=vty_int); auto.
+    rewrite Forall_forall in H.
+    simpl.
+    specialize (H (nth n vs vty_int) (ltac:(apply nth_In; auto))).
+    inversion H; auto.
+Qed.*)
+
+(*TODO: change original definition*)
+Definition upd_vv_args' pd (vt: val_typevar) (vv: val_vars pd vt)
+  p1 a1 (Hlen: length p1 = length a1)
+  (Hn: NoDup p1):
+  val_vars pd (vt_with_args vt p1 a1) :=
+  fun x =>
+  (dom_cast (dom_aux pd) 
+    (Logic.eq_sym (v_subst_vt_with_args vt p1 a1 (snd x) Hlen Hn))
+    (vv (fst x, ty_subst' p1 (sorts_to_tys a1) (snd x)))).
+
+(*Why don't we just define it the way we want?*)
+Definition upd_vv_args'' pd (vt: val_typevar) (vv: val_vars pd vt):
+  val_vars pd (vt_with_args vt params (map (v_subst vt) tys)) :=
+  fun x => 
+  (dom_cast (dom_aux pd) (v_subst_vt_with_args' vt (snd x)) 
+    (vv (ty_subst_var x))).
+
+(*TODO: these are good, move*)
+(*
+Lemma map_v_subst_sorts vt srts:
+  map (v_subst vt) (sorts_to_tys srts) = srts.
+Proof.
+  apply list_eq_ext'; rewrite !map_length; auto.
+  intros n d Hn. unfold sorts_to_tys.
+  rewrite -> !map_nth_inbound with (d2:=vty_int); auto;
+  [| rewrite map_length; auto].
+  rewrite -> map_nth_inbound with (d2:=s_int); auto.
+  apply sort_inj; simpl.
+  rewrite <- subst_is_sort_eq; auto.
+  f_equal.
+  apply nth_indep. auto.
+  destruct (nth n srts s_int); auto.
+Qed.
+
+
+Definition upd_vv_args_alt
+  (params: list typevar) (srts: list sort)
+  (lengths_eq: length params = length srts)
+  (nodup_params: NoDup params)
+  pd vt (vv: val_vars pd vt):
+  val_vars pd (vt_with_args vt params srts) :=
+  fun x =>
+  dom_cast (dom_aux pd) 
+    (f_equal (fun y => v_subst (vt_with_args vt params y) x.2) 
+      (map_v_subst_sorts vt srts))
+    (upd_vv_args'' params (sorts_to_tys srts) 
+    (eq_trans lengths_eq (Logic.eq_sym (map_length _ _))) nodup_params pd vt vv x).
+*)
+
+(*End good*)
+
+(*This lemma is still not provable (and may not be true).
+  We should use the above, and let's see what we need for 
+  function unfolding*)
+  (*
+Lemma upd_vv_args_alt_equiv params tys params_len params_nodup pd (vt: val_typevar) (vv: val_vars pd vt)
+x:
+upd_vv_args_alt params (map (v_subst vt) tys) (params_len' params tys params_len vt) params_nodup pd vt vv  
+   x =
+dom_cast (dom_aux pd) 
+  (v_subst_vt_with_args' params tys params_len params_nodup vt x)
+  (*(Logic.eq_sym (v_subst_vt_with_args vt params (map (v_subst vt) tys)
+    (snd x) (params_len' _) params_nodup)) *)
+  (vv (ty_subst_var params tys x)).
+Proof.
+  unfold upd_vv_args_alt, upd_vv_args''.
+
+  generalize dependent (map_v_subst_sorts vt (map (v_subst vt) tys)).
+  generalize dependent (sorts_to_tys (map (v_subst vt) tys)).
+  rewrite !dom_cast_compose.
+  match goal with
+  | |- dom_cast ?d ?H1 ?x1 = dom_cast ?d ?H2 ?x2 =>
+    generalize dependent H1;
+    generalize dependent H2
+  end.
+  (*Why we use this version: Only have equality of v_subst with
+    others, not underlying types*)
+  replace (sorts_to_tys (map (v_subst vt) tys)) with tys.
+  intros. apply dom_cast_eq.
+
+  rewrite map_v_subst_sorts.
+  assert (tys = )
+  generalize dependent 
+  generalize dependent (ty_subst_var params tys x).
+  assert ()
+
+
+  rewrite map_v_subst_sorts.
+
+
+
+Lemma upd_vv_args_alt_eq 
+*)
+
+ (* unfold val_vars.
+  intros Hlen Hparams. unfold val_vars in vv.
+  intros x. rewrite (v_subst_vt_with_args vt params args); 
+    [| exact Hlen | exact Hparams].
+  (*Is this a hack? Kind of*) apply (vv 
+    (fst x, (ty_subst' params (sorts_to_tys args) (snd x)))).
+Defined.*)
+(*
+Lemma dom_cast_eq d {A: Type} (g: A -> sort) 
+  (f: forall (x: A), domain d (g x)) x1 x2
+  (H1: g x1 = g x2):
+  dom_cast d H1 (f x1) = f x2.
+Proof.
+  revert H1.
+  unfold dom_cast. 
+  intros. generalize dependent (f_equal (domain d) H1).
+  intros. unfold scast. clear.
+  generalize dependent (g x2).
+  
+  revert H1. destruct e. generalize dependent (g x1). generalize dependent (domain d (g x2)).
+  generalize dependent (g x2).
+*)
+(*
+Lemma scast_eq' {A: Set} {B: A -> Set} (x1 x2: A)
+  (f: forall (x: A), B x)
+  (Hf: f x1 = f x2):
+  scast Hf (f x1) = f x2.
+  scast H1 x1 = scast H2 x2*)
+
+(*Lemma scast_eq {A B: Set} (H: A = B) (x1: A) (x2: B):
+  scast H x1 = x2.*)
+
+  (*Is this even true? The types are not the same (I think) only 
+    after v_subst, so, dont think true
+      ex: a -> int,
+        vv (x, int) and vv (x, a) not necessarily same
+        even if vt sends a -> int *)
+(*
+Lemma upd_vv_args_equiv pd (vt: val_typevar) (vv: val_vars pd vt)
+  x:
+  (upd_vv_args' pd vt vv params (map (v_subst vt) tys) 
+      (params_len' _) params_nodup) x =
+  dom_cast (dom_aux pd) 
+    (v_subst_vt_with_args' vt x)
+    (*(Logic.eq_sym (v_subst_vt_with_args vt params (map (v_subst vt) tys)
+      (snd x) (params_len' _) params_nodup)) *)
+    (vv (ty_subst_var x)).
+Proof.
+  unfold upd_vv_args'.
+  generalize dependent (v_subst_vt_with_args' vt x).
+  intros.
+  generalize dependent (v_subst_vt_with_args vt params (map (v_subst vt) tys) x.2 
+  (params_len' vt) params_nodup).
+  intros.
+  generalize dependent (v_subst (vt_with_args vt params (map (v_subst vt) tys)) x.2);
+  intros. unfold dom_cast at 2; simpl.
+  unfold ty_subst_var in *. simpl in *.
+  generalize dependent (Logic.eq_sym e0). clear e0.
+  intros.
+  generalize dependent (ty_subst' params (sorts_to_tys (map (v_subst vt) tys)) x.2).
+  generalize dependent ((ty_subst' params tys x.2)).
+  intros; subst. simpl.
+  
+  assert (vv (x.1, v0) = dom_cast (dom_aux pd) (Logic.eq_sym e0) (vv(x.1, v))).
+  unfold dom_cast. 
+  revert e. rewrite <- e0.
+  unfold dom_cast; simpl.
+  generalize dependent (v_subst vt (ty_subst' params (sorts_to_tys (map (v_subst vt) tys)) x.2)).
+
+  clear e0. rewrite <- e.
+  rewrite e0.
+  revert e.
+  rewrite e0.
+  revert e0. rewrite <- e.
+  generalize dependent e. rewrite e0.
+  generalize dependent (v_subst vt (ty_subst_var x).2).
+  unfold ty_subst_var.
+
+  rewrite e0.
+  generalize vv. unfold val_vars.
+  rewrite e0.
+  Print val_vars.
+  assert (e0 = )
+  symmetry in e, e0.
+  subst.
+  Print Ltac subst.
+  
+  subst s. unfold dom_cast. simpl.
+  unfold ty_subst_var.
+  generalize dependent (ty_subst' params (sorts_to_tys (map (v_subst vt) tys)) x.2).
+  intros.
+  generalize dependent (v_subst vt v).
+  generalize dependent ((ty_subst_var x).2).
+
+
+  subst. unfold dom_cast. simpl.
+  generalize dependent (v_subst vt (ty_subst_var x).2).
+  unfold ty_subst_var.
+  unfold eq_rec_r, dom_cast, scast. simpl.
+  unfold ty_subst_var in Heq. simpl in Heq.
+  Check (v_subst_vt_with_args vt params (map (v_subst vt) tys)
+  (snd x) (params_len' _) params_nodup).
+
+
+  vv (ty_subst_var x) = dom_cast (dom_aux pd) 
+    (v_subst_vt_with_args vt params (map (v_subst vt) tys)
+      (snd x) )
+     ( ).*)
+
+(*I think: we do need all bnd var names uniq*)
+(*y is in free vars, hmm think*)
+
+(*Lemma upd_vv_args_substi pd vt vv v x Heq y l:
+  In y l ->
+  NoDup (map fst l) ->
+  upd_vv_args'' pd vt (substi pd vt vv (ty_subst_var v) 
+    (dom_cast (dom_aux pd) Heq x)) y =
+  substi pd (vt_with_args vt params (map (v_subst vt) tys))
+    (upd_vv_args'' pd vt vv) v x y.
+Proof.
+  intros.
+  unfold substi, upd_vv_args''.
+  destruct (in_dec )
+  vsym_eq y v.
+  - vsym_eq (ty_subst_var v) (ty_subst_var v).
+    simpl.
+    assert (e = Logic.eq_refl) by (apply UIP_dec; apply vsymbol_eq_dec).
+    subst. simpl. rewrite -> dom_cast_compose, dom_cast_refl; auto.
+  - 
+  vsym_eq (ty_subst_var y) (ty_subst)
+
+
+upd_vv_args'' pd vt
+  (substi pd vt vv (ty_subst_var v)
+     (dom_cast (dom_aux pd) Heq1
+        (term_rep gamma_valid pd (vt_with_args vt params (map (v_subst vt) tys)) pf
+           (upd_vv_args'' pd vt vv) tm1 v.2 (proj1' (ty_let_inv Hty1))))) x =
+substi pd (vt_with_args vt params (map (v_subst vt) tys)) (upd_vv_args'' pd vt vv) v
+  (term_rep gamma_valid pd (vt_with_args vt params (map (v_subst vt) tys)) pf
+     (upd_vv_args'' pd vt vv) tm1 v.2 (proj1' (ty_let_inv Hty1))) x
+*)
+(*Think we need: no names in common among free vars
+  AND no names in common between free and bound vars*)
+
+(*We use a much stronger version of well-formedness:
+  No free variables have any names in common, and no
+  bound variables have names in common with free variables.
+  This doesn't cause problems, because all formulas we work
+  with are closed (or function bodies which have this restriction),
+  so we can always alpha-convert and do this.
+  TODO: actually, we can use alpha conversion in the proof,
+  so we prove for well-formed then relax that assumption by
+  alpha converting*)
+
+  Ltac simpl_forall :=
+    repeat match goal with
+    | H: Forall ?P nil |- _ => clear H
+    | H: Forall ?P (?x :: ?y) |- _ => inversion H; subst; clear H
+    | H: Forall ?P (concat ?l) |- _ => rewrite Forall_concat in H
+    | H: Forall ?P (map ?f ?l) |- _ => rewrite Forall_map in H
+    | H: Forall ?P (?l1 ++ ?l2) |- _ => rewrite Forall_app in H;
+      destruct H
+    | H: Forall ?P (?l1 ++ ?l2)%list |- _ => rewrite Forall_app in H;
+      destruct H
+    | |- Forall ?P (map ?f ?l) => rewrite Forall_map
+    end.
+
+(*Our stronger notion*)
+(*TODO: redo above (maybe others) with this*)
+Section RecHolds.
+
+Variable P_p: pattern -> Prop.
+Variable P_t: term -> Prop.
+Variable P_f: formula -> Prop.
+
+(*A condition recursively holds on all subterms and subformulas*)
+
+Fixpoint P_subpat (p: pattern) : Prop :=
+  P_p p /\
+  match p with
+  | Pconstr _ _ ps => Forall id (map P_subpat ps)
+  | Por p1 p2 => P_subpat p1 /\ P_subpat p2
+  | Pbind p v => P_subpat p
+  | _ => True
+  end.
+
+(*2 methods of this*)
+(*First, recursively holds*)
+
+Fixpoint P_subtm (t: term) : Prop :=
+  P_t t /\
+  match t with
+  | Tfun _ _ tms => Forall id (map P_subtm tms)
+  | Tlet t1 _ t2 => P_subtm t1 /\ P_subtm t2
+  | Tif f t1 t2 => P_subfmla f /\ P_subtm t1 /\ P_subtm t2
+  | Tmatch t _ ps =>
+    P_subtm t /\
+    Forall id (map (fun x => P_subpat (fst x) /\ P_subtm (snd x)) ps)
+  | Teps f _ => P_subfmla f
+  | _ => True
+  end
+with P_subfmla (f: formula) : Prop :=
+  P_f f /\
+  match f with
+  | Fpred _ _ tms => Forall id (map P_subtm tms)
+  | Feq _ t1 t2 => P_subtm t1 /\ P_subtm t2
+  | Fbinop _ f1 f2 => P_subfmla f1 /\ P_subfmla f2
+  | Fnot f => P_subfmla f
+  | Flet t1 _ f2 => P_subtm t1 /\ P_subfmla f2
+  | Fif f1 f2 f3 => P_subfmla f1 /\ P_subfmla f2 /\ P_subfmla f3
+  | Fmatch t _ ps =>
+    P_subtm t /\
+    Forall id (map (fun x => P_subpat (fst x) /\ P_subfmla (snd x)) ps)
+  | _ => True
+  end.
+
+(*Second: get all subterms/patterns/formulas*)
+Fixpoint subpats (p: pattern) : list pattern :=
+  p ::
+  match p with
+  | Pconstr _ _ ps => concat (map subpats ps)
+  | Por p1 p2 => subpats p1 ++ subpats p2
+  | Pbind p _ => subpats p
+  | _ => nil
+  end.
+
+Fixpoint subterms_t (t: term) : list term :=
+  t :: 
+  match t with
+  | Tfun _ _ tms => concat (map subterms_t tms)
+  | Tlet t1 _ t2 => subterms_t t1 ++ subterms_t t2
+  | Tif f t1 t2 => subterms_f f ++ subterms_t t1 ++ subterms_t t2
+  | Tmatch t _ ps => subterms_t t ++ 
+    concat (map (fun x => subterms_t (snd x)) ps)
+  | Teps f _ => subterms_f f
+  | _ => nil
+  end
+with subterms_f (f: formula) : list term :=
+  match f with
+  | Fpred _ _ tms => concat (map subterms_t tms)
+  | Feq _ t1 t2 => subterms_t t1 ++ subterms_t t2
+  | Fbinop _ f1 f2 => subterms_f f1 ++ subterms_f f2
+  | Fnot f => subterms_f f
+  | Flet t1 _ f2 => subterms_t t1 ++ subterms_f f2
+  | Fif f1 f2 f3 => subterms_f f1 ++ subterms_f f2 ++ subterms_f f3
+  | Fmatch t _ ps =>
+    subterms_t t ++
+    concat (map (fun x => subterms_f (snd x)) ps)
+  | _ => nil
+  end.
+
+Fixpoint subfmla_t (t: term) : list formula :=
+  match t with
+  | Tfun _ _ tms => concat (map subfmla_t tms)
+  | Tlet t1 _ t2 => subfmla_t t1 ++ subfmla_t t2
+  | Tif f t1 t2 => subfmla_f f ++ subfmla_t t1 ++ subfmla_t t2
+  | Tmatch t _ ps => subfmla_t t ++ 
+    concat (map (fun x => subfmla_t (snd x)) ps)
+  | Teps f _ => subfmla_f f
+  | _ => nil
+  end
+with subfmla_f (f: formula) : list formula :=
+  f ::
+  match f with
+  | Fpred _ _ tms => concat (map subfmla_t tms)
+  | Feq _ t1 t2 => subfmla_t t1 ++ subfmla_t t2
+  | Fbinop _ f1 f2 => subfmla_f f1 ++ subfmla_f f2
+  | Fnot f => subfmla_f f
+  | Flet t1 _ f2 => subfmla_t t1 ++ subfmla_f f2
+  | Fif f1 f2 f3 => subfmla_f f1 ++ subfmla_f f2 ++ subfmla_f f3
+  | Fmatch t _ ps =>
+    subfmla_t t ++
+    concat (map (fun x => subfmla_f (snd x)) ps)
+  | _ => nil
+  end.
+
+Fixpoint subpat_t (t: term) : list pattern :=
+  match t with
+  | Tfun _ _ tms => concat (map subpat_t tms)
+  | Tlet t1 _ t2 => subpat_t t1 ++ subpat_t t2
+  | Tif f t1 t2 => subpat_f f ++ subpat_t t1 ++ subpat_t t2
+  | Tmatch t _ ps => subpat_t t ++ 
+    concat (map (fun x => subpats (fst x) ++ subpat_t (snd x)) ps)
+  | Teps f _ => subpat_f f
+  | _ => nil
+  end
+with subpat_f (f: formula) : list pattern :=
+  match f with
+  | Fpred _ _ tms => concat (map subpat_t tms)
+  | Feq _ t1 t2 => subpat_t t1 ++ subpat_t t2
+  | Fbinop _ f1 f2 => subpat_f f1 ++ subpat_f f2
+  | Fnot f => subpat_f f
+  | Flet t1 _ f2 => subpat_t t1 ++ subpat_f f2
+  | Fif f1 f2 f3 => subpat_f f1 ++ subpat_f f2 ++ subpat_f f3
+  | Fmatch t _ ps =>
+    subpat_t t ++
+    concat (map (fun x => subpats (fst x) ++ subpat_f (snd x)) ps)
+  | _ => nil
+  end.
+
+Lemma Forall_apply {A: Type} {P Q: A -> Prop} {l}:
+  Forall P l ->
+  Forall (fun x => P x -> Q x) l ->
+  Forall Q l.
+Proof.
+  rewrite !Forall_forall; intros; auto.
+Qed.
+
+Lemma Forall_impl_in  {A: Type} {P Q: A -> Prop} {l}:
+(forall x, In x l -> P x -> Q x) ->
+Forall P l ->
+Forall Q l.
+Proof.
+  rewrite !Forall_forall; intros; auto.
+Qed.
+
+Lemma P_sub_pat_equiv1 p (Hsub: P_subpat p):
+  Forall P_p (subpats p).
+Proof.
+  induction p; simpl in *; destruct_all; try solve[repeat (constructor; auto)].
+  - constructor; auto. rewrite -> Forall_concat, Forall_map.
+    rewrite Forall_map in H1.
+    apply Forall_apply in H; auto.
+  - constructor; auto. rewrite Forall_app; split; auto.
+Qed.
+
+Lemma P_sub_equiv1 t f: 
+  (forall (Hsub: P_subtm t), Forall P_t (subterms_t t) /\
+  Forall P_f (subfmla_t t) /\ Forall P_p (subpat_t t)) /\
+  (forall (Hsub: P_subfmla f), Forall P_t (subterms_f f) /\
+  Forall P_f (subfmla_f f) /\ Forall P_p (subpat_f f)).
+Proof.
+  revert t f; apply term_formula_ind; simpl; intros;
+  destruct_all; try solve[split_all; repeat (constructor; auto)];
+  try solve[intuition; try constructor; auto; rewrite !Forall_app; auto ].
+  - rewrite Forall_map in H1.
+    apply Forall_apply in H; auto; split_all; [constructor; auto | |];
+    rewrite -> !Forall_concat, !Forall_map;
+    revert H; apply Forall_impl; intros a Hall; apply Hall.
+  - rewrite Forall_map in H3.
+    apply Forall_apply in H0; [|revert H3; rewrite Forall_map; apply Forall_impl;
+      intros a Ha; apply Ha].
+    intuition; try constructor; auto; rewrite !Forall_app; split_all; auto;
+    rewrite -> Forall_concat, Forall_map; revert H0; rewrite Forall_map; 
+    apply Forall_impl_in;
+    intros a Hina Ha; try rewrite Forall_app; try split; auto; try apply Ha.
+    apply P_sub_pat_equiv1. rewrite Forall_forall in H3; apply H3; auto.
+  - rewrite Forall_map in H1.
+    apply Forall_apply in H; auto; split_all; [|constructor; auto |];
+    rewrite -> !Forall_concat, !Forall_map;
+    revert H; apply Forall_impl; intros a Hall; apply Hall.
+  - rewrite Forall_map in H3.
+    apply Forall_apply in H0; [|revert H3; rewrite Forall_map; apply Forall_impl;
+      intros a Ha; apply Ha].
+    intuition; try constructor; auto; rewrite !Forall_app; split_all; auto;
+    rewrite -> Forall_concat, Forall_map; revert H0; rewrite Forall_map; 
+    apply Forall_impl_in;
+    intros a Hina Ha; try rewrite Forall_app; try split; auto; try apply Ha.
+    apply P_sub_pat_equiv1. rewrite Forall_forall in H3; apply H3; auto.
+Qed.
+
+
+
+Lemma P_sub_pat_equiv2 p (Hp: Forall P_p (subpats p)):
+  P_subpat p.
+Proof.
+  induction p; simpl in *; simpl_forall; split; auto; simpl_forall.
+  repeat (apply Forall_apply in H; auto).
+Qed.
+
+Lemma P_sub_equiv2 t f: 
+  (forall (Ht: Forall P_t (subterms_t t))
+    (Hf: Forall P_f (subfmla_t t))
+    (Hp: Forall P_p (subpat_t t)),
+    P_subtm t) /\
+  (forall (Ht: Forall P_t (subterms_f f))
+    (Hf: Forall P_f (subfmla_f f))
+    (Hp: Forall P_p (subpat_f f)),
+    P_subfmla f).
+Proof.
+  revert t f; apply term_formula_ind; simpl; intros;
+  simpl_forall; split; auto; simpl_forall.
+  (*Much easier to automate*)
+  - simpl_forall.
+    repeat (apply Forall_apply in H; auto).
+  - split; simpl_forall; auto.
+    apply Forall_and.
+    + revert H5. apply Forall_impl. intros. simpl_forall.
+      apply P_sub_pat_equiv2; auto.
+    + do 3(apply Forall_apply in H0; auto); auto.
+      revert H5. apply Forall_impl. intros. simpl_forall; auto.
+  - simpl_forall.
+    repeat (apply Forall_apply in H; auto).
+  - split; simpl_forall; auto.
+    apply Forall_and.
+    + revert H5. apply Forall_impl. intros. simpl_forall.
+      apply P_sub_pat_equiv2; auto.
+    + do 3(apply Forall_apply in H0; auto); auto.
+      revert H5. apply Forall_impl. intros. simpl_forall; auto.
+Qed.
+
+(*And the corollaries*)
+Lemma P_subterms_equiv t:
+  P_subtm t <-> 
+  Forall P_t (subterms_t t) /\
+  Forall P_f (subfmla_t t) /\ 
+  Forall P_p (subpat_t t).
+Proof.
+  split.
+  - apply (proj_tm P_sub_equiv1 t).
+  - intros [Ht [Hf Hp]]. apply (proj_tm P_sub_equiv2 t); auto.
+Qed.
+
+Lemma P_subfmlas_equiv f:
+  P_subfmla f <-> 
+  Forall P_t (subterms_f f) /\
+  Forall P_f (subfmla_f f) /\ 
+  Forall P_p (subpat_f f).
+Proof.
+  split.
+  - apply (proj_fmla P_sub_equiv1 f).
+  - intros [Ht [Hf Hp]]. apply (proj_fmla P_sub_equiv2 f); auto.
+Qed.
+
+(*All variables free in subterms or subformulas
+  are free or bound in original term*)
+(*Subterm formulation makes it easier to reason about
+  free variables*)
+
+Ltac simpl_in :=
+  repeat(match goal with
+  | H: In ?x (concat ?l) |- _ => rewrite in_concat in H
+  | H: In ?x (map ?f ?l) |- _ => rewrite in_map_iff in H
+  | H: In ?x ?l |- In (?f ?x) (map ?f ?l) => rewrite in_map_iff;
+    exists x; auto
+  end; destruct_all; subst); try rewrite -> !in_app_iff in *.
+
+Ltac auto_hyp :=
+  repeat match goal with
+  | H: ?P -> ?Q, H1 : ?P |- _ => specialize (H H1)
+  end; auto.
+
+Lemma subterm_fv_in x tm t f:
+  (In tm (subterms_t t) -> 
+    In x (tm_fv tm) -> In x (tm_fv t) \/
+    In x (tm_bnd t)) /\
+  (In tm (subterms_f f) -> 
+  In x (tm_fv tm) -> In x (fmla_fv f) \/
+  In x (fmla_bnd f)).
+Proof.
+  revert t f. apply term_formula_ind; simpl; intros; 
+  destruct_all; try contradiction; simpl in *;
+  destruct_all; try contradiction; subst; auto.
+  - simpl_in. simpl_set. rewrite in_concat.
+    rewrite Forall_forall in H. specialize (H _ H3 H2 H1).
+    destruct H; [left | right]; [exists x1 | exists (tm_bnd x1) ]; split; auto.
+    simpl_in.
+  - simpl_set. simpl_in. vsym_eq x v. 
+    repeat (destruct_all; auto_hyp).
+  - simpl_in. simpl_set.
+    repeat (destruct_all; auto_hyp).
+  - simpl_set. simpl_in.
+    rewrite in_concat.
+    destruct H1; [auto_hyp; destruct_all; auto_hyp| simpl_in].
+    simpl_forall. rewrite Forall_forall in H0.
+    specialize (H0 _ H4).
+    destruct (in_dec vsymbol_eq_dec x (pat_fv x1.1)).
+    + right. right. eexists. rewrite in_map_iff.
+      split. eexists. split;[reflexivity |]. apply H4.
+      simpl_in; auto.
+    + repeat (destruct_all; auto_hyp); [left | right]; right.
+      * exists x1. split; auto. simpl_set. auto.
+      * eexists. split. rewrite in_map_iff.
+        eexists. split;[reflexivity |]. apply H4.
+        simpl_in; auto.
+  - simpl_set. vsym_eq x v. repeat (destruct_all; auto_hyp).
+  - simpl_in. simpl_set. rewrite in_concat.
+    rewrite Forall_forall in H. specialize (H _ H3 H2 H1).
+    destruct H; [left | right]; [exists x1 | exists (tm_bnd x1) ]; split; auto.
+    simpl_in.
+  - simpl_in. simpl_set. repeat (destruct_all; auto_hyp).
+  - simpl_in. simpl_set. repeat (destruct_all; auto_hyp).
+  - simpl_in. simpl_set. vsym_eq x v. repeat (destruct_all; auto_hyp).
+  - simpl_in. simpl_set. repeat (destruct_all; auto_hyp).
+  - simpl_set. simpl_in.
+    rewrite in_concat.
+    destruct H1; [auto_hyp; destruct_all; auto_hyp| simpl_in].
+    simpl_forall. rewrite Forall_forall in H0.
+    specialize (H0 _ H4).
+    destruct (in_dec vsymbol_eq_dec x (pat_fv x1.1)).
+    + right. right. eexists. rewrite in_map_iff.
+      split. eexists. split;[reflexivity |]. apply H4.
+      simpl_in; auto.
+    + repeat (destruct_all; auto_hyp); [left | right]; right.
+      * exists x1. split; auto. simpl_set. auto.
+      * eexists. split. rewrite in_map_iff.
+        eexists. split;[reflexivity |]. apply H4.
+        simpl_in; auto.
+Qed.
+
+(*TODO: reflection?*)
+End RecHolds.
+
+Definition tm_wf_strong t :=
+  NoDup (map fst (tm_fv t)) /\
+  (*TODO: do we need?*)
+  NoDup (map fst (tm_bnd t)) /\
+  forall x, ~ (In x (map fst (tm_fv t))
+  /\ In x (map fst (tm_bnd t))).
+
+Definition fmla_wf_strong f :=
+  NoDup (map fst (fmla_fv f)) /\
+  NoDup (map fst (fmla_bnd f)) /\
+  forall x, ~ (In x (map fst (fmla_fv f)) /\
+    In x (map fst (fmla_bnd f))).
+
+Definition tm_wf_strong_rec := P_subtm
+  (fun _ => True) tm_wf_strong fmla_wf_strong.
+
+Definition fmla_wf_strong_rec := P_subfmla
+(fun _ => True) tm_wf_strong fmla_wf_strong.
+
+(*Plan
+  1. Prove if Nodup names of bnd, then NoDup names of bnd for all subterms/fmlas
+  2. Prove that all bnd in subterms/fmlas are in t
+  3. Use the above (plus fv lemma) to show that
+    no overlap in subterms (or else overlap in t)
+  4. Prove that if strong condition holds, no free variable dups in any
+    subterm
+  5. put together (no induction)
+  *)
+
+(*Want to show: if we have a term satisfying this condition,
+  then it satisfies it recursively*)
+  (*
+Lemma wf_strong_rec_holds t f:
+  (forall (Hwf: tm_wf_strong t), tm_wf_strong_rec t) /\
+  (forall (Hwf: fmla_wf_strong f), fmla_wf_strong_rec f).
+Proof.
+  unfold tm_wf_strong_rec, fmla_wf_strong_rec.
+  rewrite -> P_subterms_equiv, P_subfmlas_equiv. split.
+  - intros. split_all; auto. 3: rewrite Forall_forall; auto.
+    + unfold tm_wf_strong in *.
+      destruct_all.
+
+  
+  split; intros. unfold tm_wf_strong;
+  revert t f. unfold tm_wf_strong_rec, fmla_wf_strong_rec. 
+  apply term_formula_ind; simpl; intros.
+  - cbn. split; auto.
+  - cbn. split; auto.
+  - cbn. split; auto.
+    simpl_forall.
+    revert H. apply Forall_impl_in.
+    intros. apply H0.
+    clear -Hwf H.
+    unfold tm_wf_strong in *.
+    simpl in *. split_all.
+    + induction l1; simpl in *; try contradiction.
+      destruct H; subst.
+      * erewrite -> map_union  with(eq_dec2:=string_dec) in H0.
+
+
+    
+    rewrite Forall_forall; intros.
+    
+    simpl.
+
+*)
+
+(*Now prove that if a term has no duplicate bound variable
+  names and is closed, then *)
+
+
+
+(*TODO: do NOT generalize ty2*)
+(*The above works because v is bound and x is free, so
+  name cannot overlap*)
+Lemma ty_subst_tf_rep {pd: pi_dom} {pf: pi_funpred gamma_valid pd}
+  (t: term) (f: formula):
+  (forall (vt: val_typevar) (vv1: val_vars pd vt)
+    (vv2: val_vars pd (vt_with_args vt params (map (v_subst vt) tys)))
+    (ty1 ty2: vty)
+    (Hty1: term_has_type gamma t ty1)
+    (Hty2: term_has_type gamma (ty_subst_tm t) ty2)
+    (Hvv: forall x Heq, vv2 x = dom_cast (dom_aux pd) Heq 
+      (vv1 (ty_subst_var x)))
+    Heq,
+    (*[term_rep] version is ugly because of cast, but we mostly
+      need formula version (or maybe not, see)*)
+    term_rep gamma_valid pd vt pf vv1 (ty_subst_tm t) ty2 Hty2 =
+    dom_cast (dom_aux pd) Heq (term_rep gamma_valid pd 
+      (vt_with_args vt params (map (v_subst vt) tys)) pf
+      vv2
+      t ty1 Hty1)) /\
+  (forall (vt: val_typevar) (vv1: val_vars pd vt) 
+  (vv2: val_vars pd (vt_with_args vt params (map (v_subst vt) tys)))
+    (Hty1: formula_typed gamma f)
+    (Hty2: formula_typed gamma (ty_subst_fmla f))
+    (Hvv: forall x Heq, vv2 x = dom_cast (dom_aux pd) Heq 
+      (vv1 (ty_subst_var x))),
+    (*[term_rep] version is ugly because of cast, but we mostly
+      need formula version (or maybe not, see)*)
+    formula_rep gamma_valid pd vt pf vv1 (ty_subst_fmla f) Hty2 =
+    formula_rep gamma_valid pd 
+      (vt_with_args vt params (map (v_subst vt) tys)) pf
+      vv2
+      f Hty1).
+Proof.
+  revert t f. apply term_formula_ind; simpl; intros; simpl_rep_full; auto.
+  - destruct c; inversion Hty1; inversion Hty2; subst; simpl_rep_full;
+    unfold cast_dom_vty.
+    + generalize dependent ((Logic.eq_sym (ty_constint_inv Hty1))); intros.
+      assert (e = Logic.eq_refl). apply UIP_dec. apply vty_eq_dec.
+      subst. simpl. unfold dom_cast; simpl.
+      generalize dependent (Logic.eq_sym (ty_constint_inv Hty2)); intros.
+      assert (e = Logic.eq_refl). apply UIP_dec. apply vty_eq_dec.
+      subst. simpl.
+      assert ((f_equal (domain (dom_aux pd)) Heq) = Logic.eq_refl). {
+        (*NOTE: relies on UIP*)
+        apply UIP.
+      }
+      rewrite H. reflexivity.
+    + generalize dependent ((Logic.eq_sym (ty_constreal_inv Hty1))); intros.
+      assert (e = Logic.eq_refl). apply UIP_dec. apply vty_eq_dec.
+      subst. simpl. unfold dom_cast; simpl.
+      generalize dependent (Logic.eq_sym (ty_constreal_inv Hty2)); intros.
+      assert (e = Logic.eq_refl). apply UIP_dec. apply vty_eq_dec.
+      subst. simpl.
+      assert ((f_equal (domain (dom_aux pd)) Heq) = Logic.eq_refl). {
+        (*NOTE: relies on UIP*)
+        apply UIP.
+      }
+      rewrite H. reflexivity.
+  - (*Variable case - more casting*)
+    unfold var_to_dom.
+    inversion Hty1; inversion Hty2; subst.
+    rewrite Hvv. auto. intros.
+    rewrite !dom_cast_compose.
+    (*If we do not use upd_vv_args'', this is not provable*)
+    apply dom_cast_eq.
+  - (*Function case - hard because of casting already and
+    need nested inductive lemma for get_arg_list*)
+    unfold cast_dom_vty. rewrite !dom_cast_compose.
+    assert (Hmap: (map (v_subst vt) (ty_subst_list' params tys l)) =
+    (map (v_subst (vt_with_args vt params (map (v_subst vt) tys))) l)). {
+      apply list_eq_ext'; rewrite !map_length; auto.
+      intros n d Hn. unfold ty_subst_list'.
+      rewrite !map_map.
+      rewrite -> !map_nth_inbound with (d2:=vty_int); auto.
+      apply v_subst_vt_with_args'.
+    }
+    match goal with
+    | |- dom_cast ?d ?H ?x = dom_cast ?d ?H1 ?x1 =>
+      generalize dependent H; 
+      generalize dependent H1
+    end.
+    
+    assert (Hargs:
+    cast_arg_list (f_equal (sym_sigma_args f1) Hmap)
+    (fun_arg_list pd vt f1 (ty_subst_list' params tys l) (map ty_subst_tm l1)
+    (term_rep gamma_valid pd vt pf vv1) Hty2) =
+    (fun_arg_list pd (vt_with_args vt params (map (v_subst vt) tys)) f1 l l1
+        (term_rep gamma_valid pd (vt_with_args vt params (map (v_subst vt) tys)) pf
+           vv2) Hty1)).
+    {
+      unfold fun_arg_list.
+      apply (get_arg_list_vt_ext') with(s:=f1)(Heq:=Hmap);
+      rewrite map_length; auto.
+      revert H; rewrite Forall_forall; intros.
+      revert Hty0. rewrite -> map_nth_inbound with (d2:=tm_d); auto.
+      intros.
+      erewrite H; [|apply nth_In; auto |].
+      rewrite !dom_cast_compose. apply dom_cast_refl.
+      intros. apply Hvv.
+      Unshelve.
+      auto.
+    }
+    rewrite <- Hargs.
+    intros.
+    rewrite <- funs_cast_eq.
+    rewrite !dom_cast_compose. apply dom_cast_eq.
+  - (*Tlet case*)
+    assert (Heq1: v_subst (vt_with_args vt params (map (v_subst vt) tys)) v.2 =
+    v_subst vt (ty_subst' params tys v.2)).
+    {
+      symmetry; apply v_subst_vt_with_args'.
+    }
+    erewrite -> H with(vv2:=vv2)(ty1:=snd v)(Heq:=Heq1)(Hty1:=(proj1' (ty_let_inv Hty1))).
+    assert (Heq2: v_subst (vt_with_args vt params (map (v_subst vt) tys)) ty1 = v_subst vt ty2).
+    {
+      inversion Hty1; subst; inversion Hty2; subst.
+      (*Use typing*)
+      assert (ty2 = ty_subst' params tys ty1). {
+        (*TODO: import typechecker*)
+        eapply term_has_type_unique. apply H9.
+        apply ty_subst_t_ty; auto.
+        (*TODO: require*) admit.
+      }
+      subst. rewrite v_subst_vt_with_args'; auto.
+    }
+    2: { intros; apply Hvv. }
+    apply H0.
+    intros. unfold substi.
+    vsym 
+    
+    with(ty1:=ty1)(Hty1:=(proj2' (ty_let_inv Hty1)))(Heq:=Heq2).
+    (*Now we show that the inner is the same*)
+    erewrite tm_change_vv.
+    apply dom_cast_eq.
+    intros. 
+    (*TODO: how substi interacts with [upd_vv_args'']*)
+
+
+    Unshelve.
+
+
+    apply H0.
+    Unshelve.
+  assert (Heq1: v_subst vt2 (snd v) = v_subst vt1 (snd v)). {
+    eapply (@vv_cast_tm2 (Tlet tm1 v tm2) _ _ vv2 vv1); simpl; auto.
+    intros; symmetry; apply Hvt; auto.
+  }
+  rewrite H with (vv2:=vv2)(Heq:=Heq1); intros;
+  [| apply Hvt | apply Hvv]; simpl; simpl_set; auto.
+  (*Now the outer term_rep*)
+  apply H0; intros; [apply Hvt |]; simpl; simpl_set; auto.
+  (*Now have to show vv condition*)
+  unfold substi. destruct (vsymbol_eq_dec x v); subst; simpl.
+  + unfold eq_rec_r, eq_rec, eq_rect. simpl.
+    rewrite !dom_cast_compose.
+    rewrite dom_cast_refl. reflexivity.
+  + apply Hvv. simpl; simpl_set; auto. *)
+
+
+
+(*TODO: 
+  X push this fv stuff through terms and fmlas
+  X Prove typing for terms and formulas
+  Prove rep for patterns
+  Prove rep for terms and formulas
+  monomoprhic goal (maybe with )
+  Test case?
+  
+  Then unfolding*)
+
+
+  simpl.
+
+
+
+      apply (H11 i j Pwild x0 H0 H1 H2); split; auto. 
+
+
+
+  ty_subst_twice
+
+  
+  Check P_Constr.
+  
+  
+  constructor.
+  
+  
+
+  induction p.
+
+  
+    | _ => t
+  end.
+
+
+Print ty_subst.
+Print ty_subst_list.
+
 
 (*Produce proof goals for lemmas and goals*)
 Fixpoint valid_theory (t: theory) : Prop :=
